Common/CoqMaps.v
@@ -1,0 +1,10 @@
+Require Import Coq.FSets.FMapAVL.
+Require Import Coq.FSets.FMapFacts.
+Require Import Coq.Structures.OrdersEx.
+Require Import Coq.Structures.OrdersAlt.
+
+
+Module N_as_OT := Backport_OT N_as_OT.
+Module BinNatMap := FMapAVL.Make(N_as_OT).
+Module BinNatMapExtra := WProperties_fun N_as_OT BinNatMap.
+Module BinNatMapFacts := BinNatMapExtra.F.
