Common/Either.v
@@ -1,0 +1,5 @@
+Require Import Coq.Strings.String.
+
+Inductive Either {A:Type} {E:Type} : Type :=
+| Right : A  -> Either
+| Left : string -> E -> Either.
