TargetSFI/ExecutionError.v
@@ -1,10 +1,4 @@
-Require Export Lib.Monads.
-Require Import Coq.Strings.String.
-
-Require Import FunctionalExtensionality.
 Require Import TargetSFI.Machine.
-
-Set Implicit Arguments.
 
 Inductive ExecutionError :=
 | RegisterNotFound : MachineState.t -> RiscMachine.Register.t -> ExecutionError
@@ -22,45 +16,6 @@ Inductive ExecutionError :=
 | IllegalJalToZeroComponent : MachineState.t -> ExecutionError
 | IllegalJumpFromZeroComponent : MachineState.t -> ExecutionError
 .
-
-Inductive Either {A:Type} : Type :=
-| Right : A  -> Either
-| Left : string -> ExecutionError -> Either.
-
-Instance either_monad : Monad (@Either)
-  := {
-      
-      ret := fun {A:Type} (x:A) => @Right A x;
-      
-      bind := fun {A B:Type} (x : @Either A) (f : A -> @Either B) => 
-        match x with
-        | Right y => f y
-        | Left m err => Left m err
-        end
-    }.
-
-Lemma either_monad_left_id:
-  forall A B (a: A) (f: A -> @Either B),
-    bind (ret a) f = f a.
-Proof.
-  auto.
-Qed.
-
-Lemma either_monad_right_id:
-  forall A (m: @Either A),
-    bind m ret = m.
-Proof.
-  intros.
-  destruct m; auto.
-Qed.
-
-Lemma either_monad_associativity:
-  forall A B C (m: @Either A) (f: A -> @Either B) (g: B -> @Either C),
-    bind (bind m f) g = bind m (fun x => bind (f x) g).
-Proof.
-  intros.
-  destruct m; auto.
-Qed.
 
 Definition get_state (err : ExecutionError) : MachineState.t :=
   match err with
