Tests/I2MP/MP_RSC_Test.v
@@ -1,0 +1,39 @@
+Require Import Coq.Strings.String.
+Require Import Common.Either.
+Require Import Intermediate.Machine.
+
+Require Import Tests.RSC_DC_MD_Test.
+Require Import Tests.IntermediateProgramGeneration.
+
+From QuickChick Require Import QuickChick.
+Import QcDefaultNotation. Import QcNotation. Open Scope qc_scope.
+
+(* TODO *)
+(* type of the MP programs *)
+Definition mp_program := unit.
+Definition ExecutionResult := unit.
+Definition ExecutionError := unit.
+
+Definition mp_eval 
+           (p : mp_program)
+           (fuel : nat)
+  :  (@Either ExecutionResult ExecutionError)
+     * Log
+  := ((Common.Either.Left "" tt),nil).
+
+Definition CompilerError := string.
+Definition compile_program
+           `{Show CompilerError}
+           (ip : Intermediate.program)
+  : @Either mp_program CompilerError
+  := Common.Either.Left "" "".
+
+Definition mp_rsc_correct (fuel : nat) :=
+  let max_components := 4%nat in
+  rsc_correct
+    empty_cag
+    empty_dag
+    max_components
+    compile_program
+    mp_eval
+    fuel.
