Tests/I2SFI/CompilerIntegrationTests.v
@@ -5,13 +5,14 @@ Require Import Coq.NArith.BinNat.
 Require Import Coq.Lists.List.
 Require Import Coq.Strings.String.
 
+Require Import Common.Either.
+
 Require Import CompCert.Events.
 
 Require Import Source.Language.
 
 Require Import S2I.Compiler.
 Require Import I2SFI.Compiler.
-Require Import TargetSFI.EitherMonad.
 Require Import TargetSFI.Machine.
 Require Import TargetSFI.CS.
 Require Import Intermediate.Machine.
@@ -26,12 +27,12 @@ Require Import Source.Examples.NestedCalls.
 Require Import Source.Examples.Identity.
 Require Import Source.Examples.Increment.
 
-Require Import I2SFI.CompTestUtil.
 Require Import I2SFI.AbstractMachine.
-Require Import I2SFI.CompEitherMonad.
 Require Import I2SFI.CompStateMonad.
 
-Require Import TargetSFI.SFITestUtil.
+Require Import Tests.TargetSFI.SFITestUtil.
+Require Import Tests.CompTestUtil.
+Require Import Tests.I2SFI.I2SFICompUtil.
 
 From QuickChick Require Import QuickChick.
 Import QcDefaultNotation. Import QcNotation. Open Scope qc_scope.
@@ -44,13 +45,13 @@ Definition compile_and_run (sp : Source.program) (fuel : nat) :=
   | None => print_error ocaml_int_0
   | Some ip =>
     match I2SFI.Compiler.compile_program ip with
-    | CompEitherMonad.Left msg err => print_string_error (msg ++ " " ++ (show err)
+    | Common.Either.Left msg err => print_string_error (msg ++ " " ++ (show err)
                                                               ++ newline
                                                               ++ (show ip))
-    | CompEitherMonad.Right p =>
+    | Common.Either.Right p =>
       match CS.eval_program fuel p (RiscMachine.RegisterFile.reset_all) with
-      | TargetSFI.EitherMonad.Left msg err => print_error ocaml_int_1
-      | TargetSFI.EitherMonad.Right (t,(mem,_,regs)) =>
+      | Common.Either.Left msg err => print_error ocaml_int_1
+      | Common.Either.Right (t,(mem,_,regs),_) =>
         match  (RiscMachine.RegisterFile.get_register
                   RiscMachine.Register.R_COM regs) with
         | Some z =>
