Tests/I2SFI/I2SFICompUtil.v
@@ -1,0 +1,77 @@
+Require Import I2SFI.CompilerError.
+Require Import I2SFI.AbstractMachine.
+Require Import Coq.Strings.String.
+Require Import Common.CoqMaps.
+
+Require Import Tests.CompTestUtil.
+Require Import Tests.TargetSFI.SFITestUtil.
+
+From QuickChick Require Import QuickChick.
+Import QcDefaultNotation. Import QcNotation. Open Scope qc_scope.
+
+Instance show_albl : Show AbstractMachine.label :=
+  {|
+    show := fun '(n1,n2) =>
+               "("++ (show n1) ++ "," ++ (show n2) ++ ")"
+  |}.
+
+Instance show_ainstr : Show AbstractMachine.ainstr :=
+  {| show :=
+       fun i =>
+         match i with
+         | AbstractMachine.INop => "INop"
+         | AbstractMachine.ILabel lbl => ("ILabel " ++ (show lbl))
+         | AbstractMachine.IConst v r => "IConst " ++ (show v) ++ " " ++ (show r)
+         | AbstractMachine.IMov r1 r2 => "IMov " ++ (show r1) ++ " " ++ (show r2)
+         | AbstractMachine.IBinOp op r1 r2 r3 => "IBinop " ++ (show op)
+                                          ++ " " ++ (show r1)
+                                          ++ " " ++ (show r2)
+                                          ++ " " ++ (show r3)
+         | AbstractMachine.ILoad r1 r2 => "ILoad " ++ (show r1) ++ " " ++ (show r2)
+         | AbstractMachine.IStore r1 r2 => "IStore " ++ (show r1) ++ " " ++ (show r2)
+         | AbstractMachine.IBnz r l => "IBnz " ++ (show r) ++ " " ++ (show l)
+         | AbstractMachine.IJump r => "IJump " ++ (show r)
+         | AbstractMachine.IJal l => "IJal " ++ (show l)
+         | AbstractMachine.IHalt => "IHalt"
+         end
+  |}.
+
+Instance show_linstr : Show (option (list AbstractMachine.label) * AbstractMachine.ainstr) :=
+  {|
+    show :=
+      fun '(ol,i) =>
+        (show ol) ++ ":" ++ (show i)
+  |}.
+
+
+Definition show_lcode ( lcode : BinNatMap.t (BinNatMap.t AbstractMachine.lcode)) :=
+  List.fold_left
+    (fun acc1 '(cid, pmap) =>
+       List.fold_left
+         (fun acc2 '(pid, lst) =>
+            List.fold_left
+               (fun acc3 elt => acc3 ++ (show elt)  ++ newline)
+               lst (acc2 ++ "pid=" ++ (show pid) ++ newline)%string
+         ) (BinNatMap.elements pmap) (acc1 ++ "cid=" ++ (show cid) ++ newline)%string
+    ) (BinNatMap.elements lcode) EmptyString.
+
+Instance show_compiler_error : Show CompilerError :=
+  {|
+    show :=
+      fun (err:CompilerError) =>
+        match err with
+        | NoInfo => EmptyString
+        | DuplicatedLabels lcode => show_lcode lcode
+        | ExportedProcsLabelsC p1 p2 => "ExportedProcsLabelsC "
+                                                          ++ (show p1) ++ " "
+                                                          ++ (show p2) ++ " "
+        | ExportedProcsLabelsP p1 p2 p3 => "ExportedProcsLabelsP "
+                                                          ++ (show p1) ++ " "
+                                                          ++ (show p2) ++ " "
+                                                          ++ (show_map p3) ++ " "
+        | NArg p => show p
+        | TwoNArg p1 p2 => "(" ++ (show p1) ++ "," ++ (show p2) ++ ")"
+        | ProcNotImported cid pid lst =>
+          "(" ++ (show cid) ++ "," ++ (show pid) ++ ")" ++ (show lst)
+        end
+  |}.
