Tests/I2SFI/SFI_RSC_Test.v
@@ -1,0 +1,47 @@
+Require Import Coq.NArith.BinNat.
+
+Require Import Common.Either.
+Require Import TargetSFI.ExecutionError.
+
+Require Import Tests.RSC_DC_MD_Test.
+Require Import SFIPBTests.
+
+Require Import TargetSFI.Machine.
+
+Require Import I2SFI.Compiler.
+Require Import SFIPBTests.
+
+Definition update_log
+           (G : Env.t)
+           (st : MachineState.t) (t : CompCert.Events.trace)
+           (st' : MachineState.t) (log : log_type CompCert.Events.event) :=
+  let '(mem,pc,regs) := st in
+  let '(test_log,addr_log) := log in
+  let nlog :=
+      if (Nat.eqb (List.count_occ N.eq_dec addr_log pc) 0%nat)
+      then (addr_log ++ pc::nil)%list
+      else addr_log
+  in
+  match t with
+  | nil =>  (test_log,nlog)
+  | _ => ((test_log ++ t)%list,nlog)
+  end.
+
+Definition sfi_eval 
+           (p : sfi_program)
+           (fuel : nat)
+  :  (@Either (CompCert.Events.trace*MachineState.t*nat)%type ExecutionError)
+     * Log
+  := let (e,l) := (eval_program update_log p fuel) in
+     let (test_log,_) := l in
+     (e,test_log).
+
+Definition sfi_rsc_correct (fuel : nat) :=
+  let max_components := ((N.to_nat SFI.COMP_MAX) - 1)%nat in
+  rsc_correct
+    (genIConstCodeAddress CStore max_components) (* valid  jumps*)
+    (genStoreAddresConstInstr CJump max_components) (* valid pointers *)
+    max_components
+    compile_program
+    sfi_eval
+    fuel.
