Tests/I2SFI/StoreTest.v
@@ -1,35 +1,20 @@
 (**************************************************
  * Author: Ana Nora Evans (ananevans@virginia.edu)
  **************************************************)
+Require Import Coq.Bool.Bool.
 Require Import Coq.NArith.BinNat.
 Require Import Coq.ZArith.ZArith.
 Require Import Coq.Lists.List.
 Require Import Coq.Strings.String.
 
 Require Import CompCert.Events.
-
-Require Import Common.Definitions.
-Require Import Common.Maps.
-
-Require Import I2SFI.Compiler.
 Require Import TargetSFI.Machine.
-Require Import TargetSFI.EitherMonad.
-Require Import TargetSFI.StateMonad.
-Require Import TargetSFI.CS.
-Require Import TargetSFI.SFIUtil.
-Require Import TargetSFI.SFITestUtil.
-Require Import CompEitherMonad.
-Require Import CompStateMonad.
-Require Import TestIntermediate.
+Require Import TargetSFI.ExecutionError.
+Require Import Tests.TargetSFI.SFITestUtil.
+Require Import Tests.IntermediateProgramGeneration.
+Require Import Tests.CompilerPBTests.
 
-Require Import Intermediate.Machine.
-Require Import Intermediate.CS.
-
-Require Import CompTestUtil.
-Require Import I2SFI.Shrinkers.
-Require Import TargetSFI.SFITestUtil.
-Require Import I2SFI.IntermediateProgramGeneration.
-Require Import I2SFI.CompilerPBTests.
+Require Import Tests.I2SFI.SFIPBTests.
 
 From QuickChick Require Import QuickChick.
 Import QcDefaultNotation. Import QcNotation. Open Scope qc_scope.
@@ -47,12 +32,13 @@ Definition show_log_entry (entry : store_log_entry) : string :=
 Definition update_store_log
            (G : Env.t)
            (st : MachineState.t) (t : CompCert.Events.trace)
-           (st' : MachineState.t) (log : (log_type store_log_entry)) :=
+           (st' : MachineState.t)
+           (log : (log_type store_log_entry)) :=
   let '(mem,pc,regs) := st in
   let '(st_log,addr_log) := log in
   let nlog :=
       if (Nat.eqb (List.count_occ N.eq_dec addr_log pc) 0%nat)
-      then (addr_log ++ [pc])%list
+      then (addr_log ++ pc::nil)%list
       else addr_log
   in
   match RiscMachine.Memory.get_word mem pc with
@@ -62,8 +48,9 @@ Definition update_store_log
       match RiscMachine.RegisterFile.get_register rptr regs with
       | Some ptr =>
         let addr := RiscMachine.Memory.to_address ptr in
-        match RiscMachine.RegisterFile.get_register RiscMachine.Register.R_SFI_SP regs with
-        | Some sp => ((st_log ++ [(pc,addr,sp)])%list,nlog)
+        match RiscMachine.RegisterFile.get_register
+                RiscMachine.Register.R_SFI_SP regs with
+        | Some sp => ((st_log ++ (pc,addr,sp)::nil)%list,nlog)
         | _ => (st_log,nlog)
         end
       | _ => (st_log,nlog)
@@ -92,7 +79,8 @@ Instance show_store_stat : Show store_stat :=
            ++ "," ++ (show e) (* push SFI *)
   |}.
 
-Definition store_stats (log : log_type store_log_entry) (steps : nat) : store_stat :=
+Definition store_stats (log : log_type store_log_entry)
+           (steps : nat) : store_stat :=
   let '(l1,l2) := log in
   let i := (List.length (List.filter (fun '(pc,addr,sfi_sp) =>
                                         (SFI.is_same_component_bool pc addr)
@@ -101,8 +89,9 @@ Definition store_stats (log : log_type store_log_entry) (steps : nat) : store_st
            ) in
   ( steps, i, ((List.length l1) - i)%nat, List.length l2).
 
-Definition store_log_checker (log : log_type store_log_entry) (steps : nat)
-           (_: MachineState.t) :=
+Definition store_log_checker (log : log_type store_log_entry)
+           (res : CompCert.Events.trace*MachineState.t*nat) : Checker :=
+  let (_,steps) := res in
   let (l1,l2) := log in
   collect (store_stats log steps)
     match l1 with
@@ -127,7 +116,8 @@ Definition store_log_checker (log : log_type store_log_entry) (steps : nat)
                         ) l1)
     end.
 
-Definition store_log_checker_error (log : log_type store_log_entry) err :=
+Definition store_log_checker_error
+           (log : log_type store_log_entry) err :=
   match err with
   | CodeMemoryException _ _ _ =>
     whenFail "store_correct:CodeMemoryException"
@@ -135,12 +125,12 @@ Definition store_log_checker_error (log : log_type store_log_entry) err :=
   | _ => 
     whenFail
       ("TargetExecutionError:"++(show err))
-      (store_log_checker log 0%nat (get_state err))
+      (store_log_checker log ((nil,get_state err),0%nat))
   end.
 
 (*! Section prop_store_correct *) (*! extends fault_store_test *)
 Definition store_correct (fuel : nat) :=
-  check_correct TestSpecific
+  sfi_check_correct TestSpecific
                 CStore
                 update_store_log
                 store_log_checker_error
