Tests/I2SFI/Test.v
@@ -2,11 +2,11 @@ Require Import Coq.Strings.String.
 Require Import Coq.Bool.Bool.
 Require Import ZArith.
 
-Require Import I2SFI.CompilerPBTests.
-Require Import I2SFI.StoreTest.
-Require Import I2SFI.JumpTest.
-Require Import I2SFI.StackTest.
-Require Import I2SFI.RSC_DC_MD_Test.
+Require Import Tests.CompilerPBTests.
+Require Import Tests.I2SFI.StoreTest.
+Require Import Tests.I2SFI.JumpTest.
+Require Import Tests.I2SFI.StackTest.
+Require Import Tests.I2SFI.SFI_RSC_Test.
 
 From QuickChick Require Import QuickChick.
 Import QcDefaultNotation. Import QcNotation. Open Scope qc_scope.
@@ -14,7 +14,7 @@ Import QcDefaultNotation. Import QcNotation. Open Scope qc_scope.
 Require Import ExtrOcamlBasic.
 Require Import ExtrOcamlNatInt.
 
-Extract Constant Test.defNumTests => "1000".
+Extract Constant Test.defNumTests => "100".
 (* number of target machine instructions to simulate *)
 Definition FUEL := 100%nat. 
 
@@ -28,7 +28,7 @@ Definition run_stack_test :=
   show (quickCheck (stack_correct FUEL)).
 
 Definition run_rsc_test :=
-  show (quickCheck (rsc_correct FUEL)).
+  show (quickCheck (sfi_rsc_correct FUEL)).
 
 Extraction "/tmp/run_test.ml" run_store_test run_jump_test  run_stack_test run_rsc_test.
 
