Tests/TargetSFI/SFITestUtil.v
@@ -5,10 +5,12 @@ Require Import Coq.ZArith.ZArith.
 Require Import CompCert.Events.
 
 Require Import Common.Definitions.
+Require Import Common.Either.
 
 Require Import TargetSFI.Machine.
-Require Import TargetSFI.EitherMonad.
 Require Import TargetSFI.SFIUtil.
+Require Import TargetSFI.CS.
+Require Import TargetSFI.ExecutionError.
 
 From QuickChick Require Import QuickChick.
 Import QcDefaultNotation. Import QcNotation. Open Scope qc_scope.
@@ -294,5 +296,8 @@ Instance show_exec_error : Show ExecutionError :=
                 
         end                 
   |}.
+
+
+
 
 Close Scope string_scope.
